EvmCompiler/Expressions.lean
@@ -1,3 +1,5 @@
 import EvmCompiler.Expressions.Syntax
+import EvmCompiler.Expressions.EffectSemantics
 import EvmCompiler.Expressions.Semantics
 import EvmCompiler.Expressions.Compiler
+import EvmCompiler.Expressions.InteractionSemantics
